feat: update Arith

Plfl/Arith.lean
@@ -35,102 +35,106 @@ inductive Val : Tm → Prop :=
 inductive Step : Tm → Tm → Prop
   | iftru {t₂ t₃}      : Step (if true then t₂ else t₃) t₂
   | iffls {t₂ t₃}      : Step (if false then t₂ else t₃) t₃
-  | ite {t₁ t₁' t₂ t₃} : Step t₁ t₁' → Step (if t₁ then t₂ else t₃) (if t₁' then t₂ else t₃)
+  | ite {t₁ t₁' t₂ t₃} : Step t₁ t₁' →
+                          Step (if t₁ then t₂ else t₃) (if t₁' then t₂ else t₃)
   | suc {t t'}         : Step t t' → Step (succ t) (succ t')
   | prdzro             : Step (pred zero) zero
-  | prdsuc {t}         : Step (pred (succ t)) t
+  | prdsuc {t}         : Val t → Step (pred (succ t)) t
   | prd {t t'}         : Step t t' → Step (pred t) (pred t')
   | iszrozro           : Step (iszero zero) true
-  | iszrosuc {t}       : Step t zero → Step (iszero (succ t)) false
+  | iszrosuc {t}       : Val t → Step (iszero (succ t)) false
   | iszro {t t'}       : Step t t' → Step (iszero t) (iszero t')
 
-infix:40 " —→ " => Step
-
-/- Theorem: Decidability of an evaluation step -/
-theorem dec_eval_step : t —→ t' ∧ t —→ t'' → t' = t''
-  | ⟨Step.iftru, Step.iftru⟩ => rfl
-  | ⟨Step.iftru, Step.ite _⟩ => by contradiction
-  | ⟨Step.iffls, Step.iffls⟩ => rfl
-  | ⟨Step.iffls, Step.ite _⟩ => by contradiction
-  | ⟨Step.ite _, Step.iftru⟩ => by contradiction
-  | ⟨Step.ite _, Step.iffls⟩ => by contradiction
-  | ⟨Step.ite ht₁, Step.ite ht₁'⟩ => by simp [dec_eval_step ⟨ht₁, ht₁'⟩]
-  | ⟨Step.suc ht, Step.suc ht'⟩ => by simp [dec_eval_step ⟨ht, ht'⟩]
-  | ⟨Step.prdzro, Step.prdzro⟩ => rfl
-  | ⟨Step.prdzro, Step.prd _⟩ => by contradiction
-  | ⟨Step.prdsuc, Step.prdsuc⟩ => rfl
-  | ⟨Step.prdsuc, Step.prd ht'⟩ => by
-      have ht' := Step.prd ht'
-      apply @dec_eval_step (pred (succ t'))
-      apply And.intro Step.prdsuc ht'
-  | ⟨Step.prd ht, Step.prdsuc⟩ => by
-      have ht := Step.prd ht
-      apply @dec_eval_step (pred (succ t''))
-      apply And.intro ht Step.prdsuc
-  | ⟨Step.prd ht, Step.prd ht'⟩ => by simp [dec_eval_step ⟨ht, ht'⟩]
-  | ⟨Step.iszrozro, Step.iszrozro⟩ => rfl
-  | ⟨Step.iszrozro, Step.iszro _⟩ => by contradiction
-  | ⟨Step.iszrosuc _, Step.iszrosuc _⟩ => rfl
-  | ⟨Step.iszrosuc ht, Step.iszro ht'⟩ => by
-      have ht' := Step.iszro ht'
-      apply @dec_eval_step (iszero (succ _))
-      apply And.intro (Step.iszrosuc ht) ht'
-  | ⟨Step.iszro ht, Step.iszrosuc ht'⟩ => by
-      have ht := Step.iszro ht
-      apply @dec_eval_step (iszero (succ _))
-      apply And.intro ht (Step.iszrosuc ht')
-  | ⟨Step.iszro ht, Step.iszro ht'⟩ => by simp [dec_eval_step ⟨ht, ht'⟩]
+infix:40 " —⟶  " => Step
 
 /- Definition: Normal form -/
-def is_norm (t : Tm) : Prop := ∀ t', ¬ t —→ t'
+def is_norm (t : Tm) : Prop := ∀ t', ¬ t —⟶ t'
+
+/- Lemma: Contradiction of normal form -/
+theorem contra_step_norm : t —⟶ t' → is_norm t → False := by
+  intro h hn
+  simp [is_norm] at hn
+  have hn := hn t'
+  contradiction
 
 /- Theorem: All values are normal form -/
-def val_is_norm : ∀ {t}, Val t → is_norm t
+theorem val_is_norm : ∀ {t}, Val t → is_norm t
   | true , _ => by simp [is_norm]; intros t h; contradiction
   | false, _ => by simp [is_norm]; intros t h; contradiction
   | zero , _ => by simp [is_norm]; intros t h; contradiction
-  | succ n, Val.suc hn => by
+  | succ _, Val.suc hv => by
       simp [is_norm]; intros t h;
       cases h with
       | @suc _ t' h =>
-          have p := val_is_norm hn
-          simp [is_norm] at p
-          have p' := p t'
-          contradiction
+          have hn := val_is_norm hv
+          simp [contra_step_norm h hn]
+
+/- Theorem: Decidability of each evaluation step -/
+theorem dec_eval_step : t —⟶ t' → t —⟶ t'' → t' = t''
+  | Step.iftru, Step.iftru | Step.iffls, Step.iffls => rfl
+  | Step.iftru, Step.ite _ | Step.iffls, Step.ite _
+  | Step.ite _, Step.iftru | Step.ite _, Step.iffls => by contradiction
+  | Step.ite ht₁, Step.ite ht₁' => by simp [dec_eval_step ht₁ ht₁']
+  | Step.suc ht, Step.suc ht' => by simp [dec_eval_step ht ht']
+  | Step.prdzro, Step.prdzro => rfl
+  | Step.prdzro, Step.prd _ => by contradiction
+  | Step.prdsuc _, Step.prdsuc _ => rfl
+  | Step.prdsuc hv, @Step.prd _ u ht' => by
+      have hn := val_is_norm (Val.suc hv)
+      apply False.elim (contra_step_norm ht' hn)
+  | @Step.prd _ u ht, Step.prdsuc hv' => by
+      have hn := val_is_norm (Val.suc hv')
+      apply False.elim (contra_step_norm ht hn)
+  | Step.prd ht, Step.prd ht' => by simp [dec_eval_step ht ht']
+  | Step.iszrozro, Step.iszrozro => rfl
+  | Step.iszrozro, Step.iszro _ => by contradiction
+  | Step.iszrosuc _, Step.iszrosuc _ => rfl
+  | Step.iszrosuc hv, @Step.iszro _ u ht' => by
+      have hn := val_is_norm (Val.suc hv)
+      apply False.elim (contra_step_norm ht' hn)
+  | @Step.iszro _ u ht, Step.iszrosuc ht' => by
+      have hn := val_is_norm (Val.suc ht')
+      apply False.elim (contra_step_norm ht hn)
+  | Step.iszro ht, Step.iszro ht' => by simp [dec_eval_step ht ht']
 
 /- Definition: Reflexive and transitive closure of Step -/
 inductive Steps : Tm → Tm → Prop
-  | single : t —→ t' → Steps t t'
+  | single : t —⟶ t' → Steps t t'
   | refl   : ∀ {t}, Steps t t
   | trans  : Steps t t' → Steps t' t'' → Steps t t''
 
-infix:40 " —→* " => Steps
+infix:40 " —⟶* " => Steps
 
 /- Theorem: Uniqueness of normalform -/
-theorem uniq_norm : t —→* u → t —→* u' → is_norm u → is_norm u' → u = u' := by
-  intros ht ht' hn hn'
-  simp [is_norm] at hn hn'
-  induction ht generalizing u' with
-  | single h => induction ht' generalizing u with
-      | single h' => simp [dec_eval_step ⟨h, h'⟩]
-      | refl => sorry
-      | trans h₁ h₂ => sorry
-  | refl => sorry
-  | trans h₁ h₂ => sorry
+theorem uniq_norm : t —⟶* u → t —⟶* u' → is_norm u → is_norm u' → u = u'
+  | Steps.single h, Steps.single h', _, _ => by
+      simp [dec_eval_step h h']
+  | Steps.single h, Steps.refl, _, hn' => by
+      apply False.elim (contra_step_norm h hn')
+  | Steps.single h, Steps.trans h₁ h₂, hn, hn' => by
+      apply dec_eval_step h
+      sorry
+  | Steps.refl, Steps.single h', hn, _ => by
+      apply False.elim (contra_step_norm h' hn)
+  | Steps.refl, Steps.refl, _, _ => rfl
+  | Steps.refl, Steps.trans h₁' h₂', hn, hn' => sorry
+  | Steps.trans h₁ h₂, Steps.single h', hn, hn' => sorry
+  | Steps.trans h₁ h₂, Steps.refl, hn, hn' => sorry
+  | Steps.trans h₁ h₂, Steps.trans h₁' h₂', hn, hn' => sorry
 
 /- Theorem: Termination of evaluation -/
-theorem terminate_steps : ∀ t, ∃ t', is_norm t' ∧ t —→* t' := by
+theorem terminate_steps : ∀ t, ∃ t', is_norm t' ∧ t —⟶* t' := by
   intro t
   induction t with
-  | tru =>
-      exists true;
-      apply And.intro (val_is_norm Val.tru) Steps.refl
-  | fls =>
-      exists false;
-      apply And.intro (val_is_norm Val.fls) Steps.refl
+  | tru => exists true; apply And.intro (val_is_norm Val.tru) Steps.refl
+  | fls => exists false; apply And.intro (val_is_norm Val.fls) Steps.refl
   | ite t₁ t₂ t₃ ht₁ ht₂ ht₃ =>
       induction t₁ with
-      | tru => sorry
+      | tru =>
+          have ⟨t₂', ht₂⟩ := ht₂
+          exists t₂'
+          apply And.intro ht₂.left
+          sorry
       | fls => sorry
       | _ => sorry
   | zro =>
